;;; -*- Package: MKRP; Base: 10; Mode: TEXT; Syntax: Common-lisp -*-
\newlength{\premisewidth}
\newlength{\namelength}
\newlength{\usedsignlength}
\newlength{\implsignlength}
\newlength{\remainlength}
\def\implication#1#2#3#4{% 1: String max length for 2, 2: premise, 3: clause 4. impl sign
\settowidth{\premisewidth}{#1}
\setlength{\remainlength}{\textwidth}
\settowidth{\usedsignlength}{* }
\settowidth{\implsignlength}{#4}
\settowidth{\namelength}{mmmm}
\addtolength{\remainlength}{-0.5cm}
\addtolength{\remainlength}{-1\premisewidth}
\addtolength{\remainlength}{-1\namelength}
\addtolength{\remainlength}{-1\usedsignlength}
\addtolength{\remainlength}{-1\implsignlength}
\hbox to \hsize{\parbox[t]{\premisewidth}{#2} \hfil \parbox[t]{\implsignlength}{#4} \hfil #3}}




             {\bf Formulae given to the editor}

   
\parbox[t]{2cm}{Axioms:}\hfill 
\setlength{\remainlength}{\textwidth}
\addtolength{\remainlength}{-2.5cm}
\parbox[t]{\remainlength}{* AXIOMS *

             * GROUP *

             ALL X,Y,Z + (+ (X Y) Z) = + (X + (Y Z))

             ALL X + (0 X) = X

             ALL X + (- (X) X) = 0

             
}
\parbox[t]{2cm}{Theorems:}\hfill 
\setlength{\remainlength}{\textwidth}
\addtolength{\remainlength}{-2.5cm}
\parbox[t]{\remainlength}{* THEOREM *

             ALL X - (- (X)) = X

             
}


             {\bf Set of Axiom Clauses Resulting from Normalization}

           \implication{M}{}{\parbox[t]{\usedsignlength}{$  $} \hfil \parbox[t]{\namelength}{$A1$:} \hfil \parbox[t]{\remainlength}{$\forall x\in Any  (x=x)$}}{}
           \implication{M}{}{\parbox[t]{\usedsignlength}{$* $} \hfil \parbox[t]{\namelength}{$A2$:} \hfil \parbox[t]{\remainlength}{$\forall x,y,z\in Any  (((z+y)+x)=(z+(y+x)))$}}{}
           \implication{M}{}{\parbox[t]{\usedsignlength}{$* $} \hfil \parbox[t]{\namelength}{$A3$:} \hfil \parbox[t]{\remainlength}{$\forall x\in Any  ((0+x)=x)$}}{}
           \implication{M}{}{\parbox[t]{\usedsignlength}{$* $} \hfil \parbox[t]{\namelength}{$A4$:} \hfil \parbox[t]{\remainlength}{$\forall x\in Any  ((-(x)+x)=0)$}}{}
           




             {\bf Set of Theorem Clauses Resulting from Normalization}

\implication{M}{}{\parbox[t]{\usedsignlength}{$* $} \hfil \parbox[t]{\namelength}{$T5$:} \hfil \parbox[t]{\remainlength}{$\neg (-(-(c_1))=c_1)$}}{}
           

\hrule

   {\bf Refutation:}
   
   Initial Clauses: 

      \implication{M}{}{\parbox[t]{\usedsignlength}{$  $} \hfil \parbox[t]{\namelength}{$A1$:} \hfil \parbox[t]{\remainlength}{$\forall x\in Any  (x=x)$}}{}
     \implication{M}{}{\parbox[t]{\usedsignlength}{$  $} \hfil \parbox[t]{\namelength}{$A2$:} \hfil \parbox[t]{\remainlength}{$\forall x,y,z\in Any  (((z+y)+x)=(z+(y+x)))$}}{}
     \implication{M}{}{\parbox[t]{\usedsignlength}{$  $} \hfil \parbox[t]{\namelength}{$A3$:} \hfil \parbox[t]{\remainlength}{$\forall x\in Any  ((0+x)=x)$}}{}
     \implication{M}{}{\parbox[t]{\usedsignlength}{$  $} \hfil \parbox[t]{\namelength}{$A4$:} \hfil \parbox[t]{\remainlength}{$\forall x\in Any  ((-(x)+x)=0)$}}{}
     \implication{M}{}{\parbox[t]{\usedsignlength}{$  $} \hfil \parbox[t]{\namelength}{$T5$:} \hfil \parbox[t]{\remainlength}{$\neg (-(-(c_1))=c_1)$}}{}
     

   \implication{000000000000000000}{$A4,1 \land  A2,1 $}{\parbox[t]{\usedsignlength}{$* $} \hfil \parbox[t]{\namelength}{$P1$:} \hfil \parbox[t]{\remainlength}{$\forall x,y\in Any  ((0+y)=(-(x)+(x+y)))$}}{$\Rightarrow$ }
   \implication{000000000000000000}{$P1,1 \land  A3$}{\parbox[t]{\usedsignlength}{$* $} \hfil \parbox[t]{\namelength}{$RW2$:} \hfil \parbox[t]{\remainlength}{$\forall x,y\in Any  (y=(-(x)+(x+y)))$}}{$\Rightarrow$ }
   \implication{000000000000000000}{$A4,1 \land  RW2,1 $}{\parbox[t]{\usedsignlength}{$* $} \hfil \parbox[t]{\namelength}{$P4$:} \hfil \parbox[t]{\remainlength}{$\forall x\in Any  (x=(-(-(x))+0))$}}{$\Rightarrow$ }
   \implication{000000000000000000}{$P4,1 \land  RW2,1 $}{\parbox[t]{\usedsignlength}{$* $} \hfil \parbox[t]{\namelength}{$P12$:} \hfil \parbox[t]{\remainlength}{$\forall x\in Any  (0=(-(-(-(x)))+x))$}}{$\Rightarrow$ }
   \implication{000000000000000000}{$P12,1 \land  RW2,1 $}{\parbox[t]{\usedsignlength}{$* $} \hfil \parbox[t]{\namelength}{$P13$:} \hfil \parbox[t]{\remainlength}{$\forall x\in Any  (x=(-(-(-(-(x))))+0))$}}{$\Rightarrow$ }
   \implication{000000000000000000}{$P13,1 \land  P4$}{\parbox[t]{\usedsignlength}{$* $} \hfil \parbox[t]{\namelength}{$RW14$:} \hfil \parbox[t]{\remainlength}{$\forall x\in Any  (x=-(-(x)))$}}{$\Rightarrow$ }
   \implication{000000000000000000}{$RW14,1 \land  T5,1 $}{\parbox[t]{\usedsignlength}{$* $} \hfil \parbox[t]{\namelength}{$R15$:} \hfil \parbox[t]{\remainlength}{$\Box $}}{$\Rightarrow$ }
   

   \hrule

     q.e.d. 


   Time Used for Refutation: 78 seconds
