\newlength{\premisewidth}
\newlength{\namelength}
\newlength{\usedsignlength}
\newlength{\implsignlength}
\newlength{\remainlength}
\def\implication#1#2#3#4{% 1: String max length for 2, 2: premise, 3: clause 4. impl sign
\settowidth{\premisewidth}{#1}
\setlength{\remainlength}{\textwidth}
\settowidth{\usedsignlength}{* }
\settowidth{\implsignlength}{#4}
\settowidth{\namelength}{mmmm}
\addtolength{\remainlength}{-0.5cm}
\addtolength{\remainlength}{-1\premisewidth}
\addtolength{\remainlength}{-1\namelength}
\addtolength{\remainlength}{-1\usedsignlength}
\addtolength{\remainlength}{-1\implsignlength}
\hbox to \hsize{\parbox[t]{\premisewidth}{#2} \hfil \parbox[t]{\implsignlength}{#4} \hfil #3}}




             {\bf Formulae given to the editor}

   
\parbox[t]{2cm}{Axioms:}\hfill 
\setlength{\remainlength}{\textwidth}
\addtolength{\remainlength}{-2.5cm}
\parbox[t]{\remainlength}{* AXIOMS *

             * GROUP *

             ALL X,Y,Z + (+ (X Y) Z) = + (X + (Y Z))

             ALL X + (0 X) = X

             ALL X + (- (X) X) = 0

             
}
\parbox[t]{2cm}{Theorems:}\hfill 
\setlength{\remainlength}{\textwidth}
\addtolength{\remainlength}{-2.5cm}
\parbox[t]{\remainlength}{* THEOREM *

             ((ALL X,Y + (X Y) = + (Y X)) IMPL (ALL X,Y + (+ (X Y) + (X Y)) = + (+ (X X) + (Y Y))))
             AND ((ALL X,Y + (+ (X Y) + (X Y)) = + (+ (X X) + (Y Y))) IMPL (ALL X,Y - (+ (X Y)) = + (- (X) - (Y))))
             AND ((ALL X,Y - (+ (X Y)) = + (- (X) - (Y))) IMPL (ALL X,Y + (X Y) = + (Y X)))

             
}


             {\bf Set of Axiom Clauses Resulting from Normalization}

           \implication{M}{}{\parbox[t]{\usedsignlength}{$* $} \hfil \parbox[t]{\namelength}{$A1$:} \hfil \parbox[t]{\remainlength}{$\forall x\in Any  (x=x)$}}{}
           \implication{M}{}{\parbox[t]{\usedsignlength}{$* $} \hfil \parbox[t]{\namelength}{$A2$:} \hfil \parbox[t]{\remainlength}{$\forall x,y,z\in Any  (((z+y)+x)=(z+(y+x)))$}}{}
           \implication{M}{}{\parbox[t]{\usedsignlength}{$* $} \hfil \parbox[t]{\namelength}{$A3$:} \hfil \parbox[t]{\remainlength}{$\forall x\in Any  ((0+x)=x)$}}{}
           \implication{M}{}{\parbox[t]{\usedsignlength}{$* $} \hfil \parbox[t]{\namelength}{$A4$:} \hfil \parbox[t]{\remainlength}{$\forall x\in Any  ((-(x)+x)=0)$}}{}
           




             {\bf Set of Theorem Clauses Resulting from Normalization and Splitting}

   Splitpart 1
\implication{M}{ }{\parbox[t]{\usedsignlength}{$* $} \hfil \parbox[t]{\namelength}{$T5$:} \hfil \parbox[t]{\remainlength}{$\forall x,y\in Any  ((y+x)=(x+y))$}}{}
           \implication{M}{ }{\parbox[t]{\usedsignlength}{$* $} \hfil \parbox[t]{\namelength}{$T6$:} \hfil \parbox[t]{\remainlength}{$\neg (((c_2+c_1)+(c_2+c_1))=((c_2+c_2)+(c_1+c_1)))$}}{}
           

   Splitpart 2
\implication{M}{ }{\parbox[t]{\usedsignlength}{$* $} \hfil \parbox[t]{\namelength}{$T7$:} \hfil \parbox[t]{\remainlength}{$\forall x,y\in Any  (((y+x)+(y+x))=((y+y)+(x+x)))$}}{}
           \implication{M}{ }{\parbox[t]{\usedsignlength}{$* $} \hfil \parbox[t]{\namelength}{$T8$:} \hfil \parbox[t]{\remainlength}{$\neg (-((c_4+c_3))